$$

\begin{gather}

S_{4}(j) = Â (Q_2)(Q_3)(\bar{Q_1}+\bar{Q_0}) = \overline{\overline{(Q_2)(Q_3)(\bar{Q_1}+\bar{Q_0})}} = \overline{\bar{Q_{2}} + \bar{Q_{3}} + \overline{(\bar{Q_1}+\bar{Q_0})}}\\

S_{4}(k) = 1 \\

S_{3}(j) = Q_{2} \\

S_{3}(k) = Q_{2} \\

S_{2}(j) = \bar{Q_{4}} \\

S_{2}(k) = 1 \\

S_{1}(j) = (Q_{0})(Q_{4}) = \overline{\bar{Q_{0}} + \bar{Q_{4}}}\\

S_{1}(k) = (Q_{0})(Q_{2})(Q_{3}) = \overline{\bar{Q_{0}} + \bar{Q_{2}} + \bar{Q_{3}}}\\

S_{0}(j) = (Q_{4}) \\

S_{0}(k) = (Q_{3}+\bar{Q_{2}})(Q_{2} + \bar{Q_{1}})(Q_{4} + Q_{1}) = \overline{\overline{(Q_{3}+\bar{Q_{2}})(Q_{2} + \bar{Q_{1}})(Q_{4} + Q_{1})}} = \overline{\overline{(Q_{3}+\bar{Q_{2}})} + \overline{(Q_{2} + \bar{Q_{1}})} + \overline{(Q_{4} + Q_{1})}} \\

\end{gather}

$$
