
4
$$

Q_4^{'} = Q_3Q_2\bar{Q_1} + Q_3Q_2\bar{Q_0} = Q_4^{'} = \overline{ \overline{ Q_3Q_2\bar{Q_1} } \& \overline{ Q_3Q_2\bar{Q_0} } }\\
$$
3
$$
Q_3^{'} = Q_3\bar{Q_2} + \bar{Q_3}Q_2 = Q_3^{'} = \overline{ \overline{ Q_3\bar{Q_2} } \& \overline{ \bar{Q_3}Q_2 } } \\
$$
2
$$
Q_2^{'} = \bar{Q_4}\bar{Q_2} \\
$$
1
$$
Q_1^{'} = Q_4Q_0 + Q_1\bar{Q_0} +\bar{Q_2}Q_1 + \bar{Q_3}Q_1 = Q_1^{'} = \overline{ \overline{ Q_4Q_0 } \& \overline{ Q_1\bar{Q_0} } \& \overline{ \bar{Q_2}Q_1 } \& \overline{ \bar{Q_3}Q_1 } } \\
$$
0
$$
Q_0^{'} = Q_4\bar{Q_0} + \bar{Q_3}Q_2Q_0 + \bar{Q_2}Q_{1}Q_{0} + \bar{Q_{4}}\bar{Q_{1}}Q_{0} = Q_0^{'} = \overline{ \overline{ Q_4\bar{Q_0} } \& \overline{ \bar{Q_3}Q_2Q_0 } \& \overline{ \bar{Q_2}Q_{1}Q_{0} } \& \overline{ \bar{Q_{4}} \bar{Q_{1}}Q_{0} } }
$$